\newcommand*{\titleContent}{与《数理逻辑》相配套的一些证明和演绎}
\newif\ifbsixpaper
% \bsixpapertrue
\ifbsixpaper
\documentclass[punct=custom/kaiming,fontset=none]{ctexart}
\usepackage[b6paper,hmargin=.4in,vmargin=.3in]{geometry}
\title{\Large\bfseries\titleContent}
\else
\documentclass[a4paper,punct=custom/kaiming,fontset=none]{ctexart}
\usepackage[hmargin=1in,vmargin=1in]{geometry}
\title{\bfseries\titleContent}
\fi

\newcommand*{\authorContent}{赵磊}
\author{\authorContent}

\usepackage{mathtools,amssymb,amsthm}
\newcommand\SetSymbol[1][]{%
  \nonscript\:#1\vert
  \allowbreak
  \nonscript\:
  \mathopen{}}
% \DeclarePairedDelimiterX{\paren}[1]{\lparen}{\rparen}{%
%   \renewcommand{\given}{\SetSymbol[\delimsize]}#1}
\DeclarePairedDelimiterX{\brce}[1]{\lbrace}{\rbrace}{%
  \newcommand*{\given}{\SetSymbol[\delimsize]}#1}
\usepackage{lualatex-math}

\newif\ifadobe
% \adobetrue

\ifadobe
\setmainfont{Latin Modern Roman}[BoldFont=Adobe Heiti Std]
\setCJKmainfont{Adobe Song Std}[
  BoldFont=Adobe Heiti Std,
  ItalicFont=Adobe Kaiti Std
]
\else
\setmainfont{Times New Roman}[BoldFont=Heiti SC,Ligatures=Rare]
\setCJKmainfont{Songti SC}[BoldFont=Heiti SC,ItalicFont=Kaiti SC]
\usepackage[
  math-style=TeX,
  warnings-off={mathtools-colon,mathtools-overbracket}
]{unicode-math}
\setmathfont{Asana Math}
% \setmathfont{STIX Two Math}[range="002C]
\fi

\newcommand*{\enumparen}[1]{\textnormal{（}\makebox[0.5em][c]{#1}\textnormal{）}}

% https://www.logicmatters.net/resources/nd3.sty
% https://www.logicmatters.net/resources/pdfs/nd-manual2a.pdf
\usepackage{nd3}
\renewcommand*{\ndstretch}{.25}

\usepackage{xcolor}
\usepackage[
  pdftitle={\titleContent},
  pdfauthor={\authorContent},
  hyperfootnotes=false,
  colorlinks=true,
  urlcolor={.},
  linkcolor={.}
]{hyperref}

\makeatletter
\newcommand*{\theH@NDlines}{\@NDident.\number\value{@NDlines}}
\makeatother

\AtBeginDocument{%
  % \renewcommand{\perp}{\mathrel{\bot}}
  \let\oldref\ref
  \let\proves\vdash
  \let\leq\leqslant
  \let\le\leq
  \let\geq\geqslant
  \let\ge\geq
}

\begin{document}
\maketitle

\begin{enumerate}
\item \label{thm:iden} \(\proves \phi \to \phi\)
  \begin{ND}[][][][\rwidth{ded:wedgeComm1}]
    \ndl{}{\(\phi \to (\phi \to \phi) \to \phi\)}{\(\rm P_1\)}\label{1}
    \ndl{}{\((\phi \to (\phi \to \phi) \to \phi) \to (\phi \to \phi \to \phi) \to (\phi \to \phi)\)}{\(\rm P_2\)}\label{2}
    \ndl{}{\(\phi \to \phi \to \phi\)}{\(\rm P_1\)}\label{3}
    \ndl{}{\((\phi \to \phi \to \phi) \to (\phi \to \phi)\)}{\ref{1}，\ref{2}，MP}\label{4}
    \ndl{}{\(\phi \to \phi\)}{\ref{3}，\ref{4}，MP}
  \end{ND}
\item \label{thm:abcb} \(\proves \phi \to \psi \to \theta \to \psi\)
  \begin{ND}[][][][\rwidth{ded:wedgeComm1}]
    \ndl{}{\(\psi \to \theta \to \psi\)}{\(\rm P_1\)}\label{1}
    \ndl{}{\((\psi \to \theta \to \psi) \to \phi \to (\psi \to \theta \to \psi)\)}{\(\rm P_1\)}\label{2}
    \ndl{}{\(\phi \to \psi \to \theta \to \psi\)}{\ref{1}，\ref{2}，MP}
  \end{ND}
\item \label{ded:axiom1} \(\phi \proves \psi \to \phi\)
  \begin{ND}[][][][\rwidth{ded:wedgeComm1}]
    \ndl{}{\(\phi\)}{假设}\label{1}
    \ndl{}{\(\phi \to \psi \to \phi\)}{\(\rm P_1\)}\label{2}
    \ndl{}{\(\psi \to \phi\)}{\ref{1}，\ref{2}，MP}
  \end{ND}
\item \label{ded:axiom2} \(\phi \to \psi \to \theta,\ \psi \proves \phi \to \theta\)
  \begin{ND}[][][][\rwidth{ded:wedgeComm1}]
    \ndl{}{\(\phi \to \psi \to \theta\)}{假设}\label{1}
    \ndl{}{\((\phi \to \psi \to \theta) \to (\phi \to \psi) \to (\phi \to \theta)\)}{\(\rm P_2\)}\label{2}
    \ndl{}{\(\psi\)}{假设}\label{3}
    \ndl{}{\(\phi \to \psi\)}{\ref{3}，演绎\oldref{ded:axiom1}}\label{4}
    \ndl{}{\((\phi \to \psi) \to (\phi \to \theta)\)}{\ref{1}，\ref{2}，MP}\label{5}
    \ndl{}{\(\phi \to \theta\)}{\ref{4}，\ref{5}，MP}
  \end{ND}
\item \label{ded:axiom2add} \(\phi \to \theta \proves \phi \to \psi \to \theta\)
  \begin{ND}[][][][\rwidth{ded:wedgeComm1}]
    \ndl{}{\(\phi \to \theta \to \psi \to \theta\)}{证明\oldref{thm:abcb}}\label{1}
    \ndl{}{\((\phi \to \theta \to \psi \to \theta) \to (\phi \to \theta) \to (\phi \to \psi \to \theta)\)}{\(\rm P_1\)}\label{2}
    \ndl{}{\(\phi \to \theta\)}{假设}\label{3}
    \ndl{}{\((\phi \to \theta) \to (\phi \to \psi \to \theta)\)}{\ref{1}，\ref{2}，MP}\label{4}
    \ndl{}{\(\phi \to \psi \to \theta\)}{\ref{3}，\ref{4}，MP}
  \end{ND}
\item \label{ded:comm} \(\phi \to \psi \to \theta \proves \psi \to \phi \to \theta\)
  \begin{ND}[][][][\rwidth{ded:wedgeComm1}]
    \ndl{}{\(\phi \to \psi \to \theta\)}{假设}\label{1}
    \ndl{}{\((\phi \to \psi \to \theta) \to (\phi \to \psi) \to (\phi \to \theta)\)}{\(\rm P_2\)}\label{2}
    \ndl{}{\((\phi \to \psi) \to (\phi \to \theta)\)}{\ref{1}，\ref{2}，MP}\label{3}
    \ndl{}{\(\psi \to (\phi \to \psi) \to (\phi \to \theta)\)}{\ref{3}，演绎\oldref{ded:axiom1}}\label{4}
    \ndl{}{\((\psi \to (\phi \to \psi) \to (\phi \to \theta)) \to (\psi \to (\phi \to \psi)) \to (\psi \to (\phi \to \theta))\)}{\(\rm P_2\)}\label{5}
    \ndl{}{\(\psi \to \phi \to \psi\)}{\(\rm P_1\)}\label{6}
    \ndl{}{\((\psi \to \phi \to \psi) \to (\psi \to \phi \to \theta)\)}{\ref{4}，\ref{5}，MP}\label{7}
    \ndl{}{\(\psi \to \phi \to \theta\)}{\ref{6}，\ref{7}，MP}
  \end{ND}
\item \label{ded:trans} \(\phi \to \psi,\ \psi \to \theta \proves \phi \to \theta\)
  \begin{ND}[][][][\rwidth{ded:wedgeComm1}]
    \ndl{}{\(\psi \to \theta\)}{假设}\label{1}
    \ndl{}{\((\psi \to \theta) \to \phi \to (\psi \to \theta)\)}{\(\rm P_1\)}\label{2}
    \ndl{}{\(\phi \to \psi \to \theta\)}{\ref{1}，\ref{2}，MP}\label{3}
    \ndl{}{\((\phi \to \psi \to \theta) \to (\phi \to \psi) \to (\phi \to \theta)\)}{\(\rm P_2\)}\label{4}
    \ndl{}{\(\phi \to \psi\)}{假设}\label{5}
    \ndl{}{\((\phi \to \psi) \to (\phi \to \theta)\)}{\ref{3}，\ref{4}，MP}\label{6}
    \ndl{}{\(\phi \to \theta\)}{\ref{5}，\ref{6}，MP}
  \end{ND}
\item \label{thm:trans} \(\proves (\phi \to \psi) \to (\psi \to \theta) \to (\phi \to \theta)\)
  \begin{ND}[][thm:trans][][\rwidth{ded:wedgeComm1}]
    \ndl{}{\((\psi \to \theta) \to \phi \to (\psi \to \theta)\)}{\(\rm P_1\)}\label{1}
    \ndl{}{\((\phi \to \psi \to \theta) \to (\phi \to \psi) \to (\phi \to \theta)\)}{\(\rm P_2\)}\label{2}
    \ndl{}{\((\psi \to \theta) \to (\phi \to \psi) \to (\phi \to \theta)\)}{\ref{1}，\ref{2}，演绎\oldref{ded:trans}}\label{3}
    \ndl{}{\((\phi \to \psi) \to (\psi \to \theta) \to (\phi \to \theta)\)}{\ref{3}，演绎\oldref{ded:comm}}
  \end{ND}
\item \label{ded:mp} \(\phi,\ \phi \to \psi \proves \psi\)
  \begin{ND}[][][][\rwidth{ded:wedgeComm1}]
    \ndl{}{\(\phi\)}{假设}\label{1}
    \ndl{}{\(\phi \to \psi\)}{假设}\label{2}
    \ndl{}{\(\psi\)}{\ref{1}，\ref{2}，MP}
  \end{ND}
\item \label{thm:mpAux} \(\proves ((\phi \to \psi) \to \phi) \to ((\phi \to \psi) \to \psi)\)
  \begin{ND}[][][][\rwidth{ded:wedgeComm1}]
    \ndl{}{\((\phi \to \psi) \to (\phi \to \psi)\)}{证明\oldref{thm:iden}}\label{1}
    \ndl{}{\(((\phi \to \psi) \to \phi \to \psi) \to ((\phi \to \psi) \to \phi) \to ((\phi \to \psi) \to \psi)\)}{\(\rm P_2\)}\label{2}
    \ndl{}{\(((\phi \to \psi) \to \phi) \to ((\phi \to \psi) \to \psi)\)}{\ref{1}，\ref{2}，MP}
  \end{ND}
\item \label{ded:mp1} \(\phi \proves (\phi \to \psi) \to \psi\)
  \begin{ND}[][][][\rwidth{ded:wedgeComm1}]
    \ndl{}{\(\phi\)}{假设}\label{1}
    \ndl{}{\((\phi \to \psi) \to \phi\)}{\ref{1}，演绎\oldref{ded:axiom1}}\label{2}
    \ndl{}{\(((\phi \to \psi) \to \phi) \to ((\phi \to \psi) \to \psi)\)}{证明\oldref{thm:mpAux}}\label{3}
    \ndl{}{\((\phi \to \psi) \to \psi\)}{\ref{2}，\ref{3}，MP}
  \end{ND}
\item \label{thm:mp} \(\proves \phi \to (\phi \to \psi) \to \psi\)
  \begin{ND}[][][][\rwidth{ded:wedgeComm1}]
    \ndl{}{\(\phi \to (\phi \to \psi) \to \phi\)}{\(\rm P_1\)}\label{1}
    \ndl{}{\(((\phi \to \psi) \to \phi) \to ((\phi \to \psi) \to \psi)\)}{证明\oldref{thm:mpAux}}\label{2}
    \ndl{}{\(\phi \to (\phi \to \psi) \to \psi\)}{\ref{1}，\ref{2}，演绎\oldref{ded:trans}}
  \end{ND}
\item \label{ded:axiom3alt} \(\neg\phi \to \neg\psi \proves \psi \to \phi\)
  \begin{ND}[][][][\rwidth{ded:wedgeComm1}]
    \ndl{}{\(\neg\phi \to \neg\psi\)}{假设}\label{1}
    \ndl{}{\((\neg\phi \to \neg\psi) \to (\neg\phi \to \psi) \to \phi\)}{\(\rm P_3\)，演绎\oldref{ded:comm}}\label{2}
    \ndl{}{\(\psi \to (\neg\phi \to \psi)\)}{\(\rm P_1\)}\label{3}
    \ndl{}{\((\neg\phi \to \psi) \to \phi\)}{\ref{1}，\ref{2}，MP}\label{4}
    \ndl{}{\(\psi \to \phi\)}{\ref{3}，\ref{4}，演绎\oldref{ded:trans}}
  \end{ND}
\item \label{thm:axiom3alt} \(\proves (\neg\phi \to \neg\psi) \to (\psi \to \phi)\)
  \begin{ND}[][][][\rwidth{ded:wedgeComm1}]
    \ndl{}{\((\neg\phi \to \neg\psi) \to (\neg\phi \to \psi) \to \phi\)}{\(\rm P_3\)，演绎\oldref{ded:comm}}\label{1}
    \ndl{}{\((\neg\phi \to \neg\psi) \to \psi \to (\neg\phi \to \psi) \to \phi\)}{\ref{1}，演绎\oldref{ded:axiom2add}}\label{2}
    \ndl{}{\((\psi \to (\neg\phi \to \psi) \to \phi) \to (\psi \to \neg\phi \to \psi) \to (\psi \to \phi)\)}{\(\rm P_2\)}\label{3}
    \ndl{}{\((\neg\phi \to \neg\psi) \to (\psi \to \neg\phi \to \psi) \to (\psi \to \phi)\)}{\ref{2}，\ref{3}，演绎\oldref{ded:trans}}\label{4}
    \ndl{}{\(\psi \to \neg\phi \to \psi\)}{\(\rm P_1\)}\label{5}
    \ndl{}{\((\neg\phi \to \neg\psi) \to (\psi \to \phi)\)}{\ref{4}，\ref{5}，演绎\oldref{ded:axiom2}}
  \end{ND}
  或者
  \begin{ND}[][][][\rwidth{ded:wedgeComm1}]
    \ndl{}{\(\psi \to (\neg\phi \to \psi)\)}{\(\rm P_1\)}\label{1}
    \ndl{}{\((\neg\phi \to \psi) \to (\neg\phi \to \neg\psi) \to \phi\)}{\(\rm P_3\)}\label{2}
    \ndl{}{\(\psi \to (\neg\phi \to \neg\psi) \to \phi\)}{\ref{1}，\ref{2}，演绎\oldref{ded:trans}}\label{3}
    \ndl{}{\((\neg\phi \to \neg\psi) \to (\psi \to \phi)\)}{\ref{3}，演绎\oldref{ded:comm}}
  \end{ND}
\item \label{ded:dnOut} \(\neg\neg\phi \proves \phi\)
  \begin{ND}[][][][\rwidth{ded:wedgeComm1}]
    \ndl{}{\(\neg\neg\phi\)}{假设}\label{1}
    \ndl{}{\(\neg\phi \to \neg\phi\)}{证明\oldref{thm:iden}}\label{2}
    \ndl{}{\((\neg\phi \to \neg\phi) \to (\neg\phi \to \neg\neg\phi) \to \phi\)}{\(\rm P_3\)}\label{3}
    \ndl{}{\(\neg\phi \to \neg\neg\phi\)}{\ref{1}，演绎\oldref{ded:axiom1}}\label{4}
    \ndl{}{\((\neg\phi \to \neg\neg\phi) \to \phi\)}{\ref{2}，\ref{3}，MP}\label{5}
    \ndl{}{\(\phi\)}{\ref{4}，\ref{5}，MP}
  \end{ND}
\item \label{thm:dnOut} \(\proves \neg\neg\phi \to \phi\)
  \begin{ND}[][][][\rwidth{ded:wedgeComm1}]
    \ndl{}{\(\neg\phi \to \neg\phi\)}{证明\oldref{thm:iden}}\label{1}
    \ndl{}{\((\neg\phi \to \neg\phi) \to (\neg\phi \to \neg\neg\phi) \to \phi\)}{\(\rm P_3\)}\label{2}
    \ndl{}{\(\neg\neg\phi \to (\neg\phi \to \neg\neg\phi)\)}{\(\rm P_1\)}\label{3}
    \ndl{}{\((\neg\phi \to \neg\neg\phi) \to \phi\)}{\ref{1}，\ref{2}，MP}\label{4}
    \ndl{}{\(\neg\neg\phi \to \phi\)}{\ref{3}，\ref{4}，演绎\oldref{ded:trans}}
  \end{ND}
\item \label{thm:dnInAnte} \(\proves (\phi \to \psi) \to (\neg\neg\phi \to \psi)\)
  \begin{ND}[][][][\rwidth{ded:wedgeComm1}]
    \ndl{}{\(\neg\neg\phi \to \phi\)}{证明\oldref{thm:dnOut}}\label{1}
    \ndl{}{\((\neg\neg\phi \to \phi) \to (\phi \to \psi) \to (\neg\neg\phi \to \psi)\)}{证明\oldref{thm:trans}}\label{2}
    \ndl{}{\((\phi \to \psi) \to (\neg\neg\phi \to \psi)\)}{\ref{1}，\ref{2}，MP}
  \end{ND}
\item \label{ded:dnInAnte} \(\phi \to \psi \proves \neg\neg\phi \to \psi\)
  \begin{ND}[][][][\rwidth{ded:wedgeComm1}]
    \ndl{}{\(\phi \to \psi\)}{假设}\label{1}
    \ndl{}{\((\phi \to \psi) \to (\neg\neg\phi \to \psi)\)}{证明\oldref{thm:dnInAnte}}\label{2}
    \ndl{}{\(\neg\neg\phi \to \psi\)}{\ref{1}，\ref{2}，MP}
  \end{ND}
\item \label{thm:axiom3in} \(\proves (\phi \to \psi) \to (\phi \to \neg\psi) \to \neg\phi\)
  \begin{ND}[][][][\rwidth{ded:wedgeComm1}]
    \ndl{}{\((\phi \to \neg\psi) \to (\neg\neg\phi \to \neg\psi)\)}{证明\oldref{thm:dnInAnte}}\label{1}
    \ndl{}{\((\neg\neg\phi \to \neg\psi) \to (\neg\neg\phi \to \psi) \to \neg\phi\)}{\(\rm P_3\)，演绎\oldref{ded:comm}}\label{2}
    \ndl{}{\((\phi \to \neg\psi) \to (\neg\neg\phi \to \psi) \to \neg\phi\)}{\ref{1}，\ref{2}，演绎\oldref{ded:trans}}\label{3}
    \ndl{}{\((\phi \to \psi) \to (\neg\neg\phi \to \psi)\)}{证明\oldref{thm:dnInAnte}}\label{4}
    \ndl{}{\((\neg\neg\phi \to \psi) \to (\phi \to \neg\psi) \to \neg\phi\)}{\ref{3}，演绎\oldref{ded:comm}}\label{5}
    \ndl{}{\((\phi \to \psi) \to (\phi \to \neg\psi) \to \neg\phi\)}{\ref{4}，\ref{5}，MP}
  \end{ND}
\item \label{ded:dnIn} \(\phi \proves \neg\neg\phi\)
  \begin{ND}[][][][\rwidth{ded:wedgeComm1}]
    \ndl{}{\(\phi\)}{假设}\label{1}
    \ndl{}{\(\neg\phi \to \phi\)}{\ref{1}，演绎\oldref{ded:axiom1}}\label{2}
    \ndl{}{\((\neg\phi \to \phi) \to (\neg\phi \to \neg\phi) \to \neg\neg\phi\)}{证明\oldref{thm:axiom3in}}\label{3}
    \ndl{}{\(\neg\phi \to \neg\phi\)}{证明\oldref{thm:iden}}\label{4}
    \ndl{}{\((\neg\phi \to \neg\phi) \to \neg\neg\phi\)}{\ref{2}，\ref{3}，MP}\label{5}
    \ndl{}{\(\neg\neg\phi\)}{\ref{4}，\ref{5}，MP}
  \end{ND}
\item \label{thm:dnIn} \(\proves \phi \to \neg\neg\phi\)
  \begin{ND}[][][][\rwidth{ded:wedgeComm1}]
    \ndl{}{\(\phi \to (\neg\phi \to \phi)\)}{\(\rm P_1\)}\label{1}
    \ndl{}{\((\neg\phi \to \phi) \to (\neg\phi \to \neg\phi) \to \neg\neg\phi\)}{证明\oldref{thm:axiom3in}}\label{2}
    \ndl{}{\(\phi \to (\neg\phi \to \neg\phi) \to \neg\neg\phi\)}{\ref{1}，\ref{2}，演绎\oldref{ded:trans}}\label{3}
    \ndl{}{\(\neg\phi \to \neg\phi\)}{证明\oldref{thm:iden}}\label{4}
    \ndl{}{\(\phi \to \neg\neg\phi\)}{\ref{3}，\ref{4}，演绎\oldref{ded:axiom2}}
  \end{ND}
\item \label{thm:dnInConseq} \(\proves (\phi \to \psi) \to (\phi \to \neg\neg\psi)\)
  \begin{ND}[][][][\rwidth{ded:wedgeComm1}]
    \ndl{}{\(\psi \to \neg\neg\psi\)}{证明\oldref{thm:dnIn}}\label{1}
    \ndl{}{\(\phi \to \psi \to \neg\neg\psi\)}{演绎\oldref{ded:axiom1}}\label{2}
    \ndl{}{\((\phi \to \psi \to \neg\neg\psi) \to (\phi \to \psi) \to (\phi \to \neg\neg\psi)\)}{\(\rm P_2\)}\label{3}
    \ndl{}{\((\phi \to \psi) \to (\phi \to \neg\neg\psi)\)}{\ref{2}，\ref{3}，MP}
  \end{ND}
\item \label{ded:dnInConseq} \(\phi \to \psi \proves \phi \to \neg\neg\psi\)
  \begin{ND}[][][][\rwidth{ded:wedgeComm1}]
    \ndl{}{\(\phi \to \psi\)}{假设}\label{1}
    \ndl{}{\((\phi \to \psi) \to (\phi \to \neg\neg\psi)\)}{证明\oldref{thm:dnInConseq}}\label{2}
    \ndl{}{\(\phi \to \neg\neg\psi\)}{\ref{1}，\ref{2}，MP}
  \end{ND}
\item \label{ded:wedgeIn} \(\phi,\ \psi \proves \phi \land \psi\)
  \begin{ND}[][][][\rwidth{ded:wedgeComm1}]
    \ndl{}{\(\psi\)}{假设}\label{1}
    \ndl{}{\(((\phi \to \neg\psi) \to \psi)\)}{\ref{1}，演绎\oldref{ded:axiom1}}\label{2}
    \ndl{}{\(((\phi \to \neg\psi) \to \psi) \to ((\phi \to \neg\psi) \to \neg\psi) \to \neg(\phi \to \neg\psi)\)}{证明\oldref{thm:axiom3in}}\label{3}
    \ndl{}{\(\phi\)}{假设}\label{4}
    \ndl{}{\(\phi \to (\phi \to \neg\psi) \to \neg\psi\)}{证明\oldref{thm:mp}}\label{5}
    \ndl{}{\((\phi \to \neg\psi) \to \neg\psi\)}{\ref{4}，\ref{5}，MP}\label{6}
    \ndl{}{\(((\phi \to \neg\psi) \to \neg\psi) \to \neg(\phi \to \neg\psi)\)}{\ref{2}，\ref{3}，MP}\label{7}
    \ndl{}{\(\neg(\phi \to \neg\psi)\)}{\ref{6}，\ref{7}，MP}\label{8}
    \ndl{}{\(\phi \land \psi\)}{\ref{8}，定义2.2.4}
  \end{ND}
\item \label{ded:exFalso} \(\phi,\ \neg\phi \proves \psi\)
  \begin{ND}[][][][\rwidth{ded:wedgeComm1}]
    \ndl{}{\(\phi\)}{假设}\label{1}
    \ndl{}{\(\neg\psi \to \phi\)}{\ref{1}，演绎\oldref{ded:axiom1}}\label{2}
    \ndl{}{\((\neg\psi \to \phi) \to (\neg\psi \to \neg\phi) \to \psi\)}{\(\rm P_3\)}\label{3}
    \ndl{}{\(\neg\phi\)}{假设}\label{4}
    \ndl{}{\(\neg\psi \to \neg\phi\)}{\ref{4}，演绎\oldref{ded:axiom1}}\label{5}
    \ndl{}{\((\neg\psi \to \neg\phi) \to \psi\)}{\ref{2}，\ref{3}，MP}\label{6}
    \ndl{}{\(\psi\)}{\ref{5}，\ref{6}，MP}
  \end{ND}
\item \label{thm:exFalso} \(\proves \phi \to \neg\phi \to \psi\)
  \begin{ND}[][][][\rwidth{ded:wedgeComm1}]
    \ndl{}{\(\phi \to (\neg\psi \to \phi)\)}{\(\rm P_1\)}\label{1}
    \ndl{}{\((\neg\psi \to \phi) \to (\neg\psi \to \neg\phi) \to \psi\)}{\(\rm P_3\)}\label{2}
    \ndl{}{\(\phi \to (\neg\psi \to \neg\phi) \to \psi\)}{\ref{1}，\ref{2}，演绎\oldref{ded:trans}}\label{3}
    \ndl{}{\(\neg\phi \to (\neg\psi \to \neg\phi)\)}{\(\rm P_1\)}\label{4}
    \ndl{}{\((\neg\psi \to \neg\phi) \to \phi \to \psi\)}{\ref{3}，演绎\oldref{ded:comm}}\label{5}
    \ndl{}{\(\neg\phi \to \phi \to \psi\)}{\ref{4}，\ref{5}，演绎\oldref{ded:trans}}\label{6}
    \ndl{}{\(\phi \to \neg\phi \to \psi\)}{\ref{6}，演绎\oldref{ded:comm}}
  \end{ND}
\item \label{ded:wedgeOutRight} \(\phi \land \psi \proves \psi\)
  \begin{ND}[][][][\rwidth{ded:wedgeComm1}]
    \ndl{}{\(\phi \land \psi\)}{假设}\label{1}
    \ndl{}{\(\neg(\phi \to \neg\psi)\)}{\ref{1}，定义2.2.4}\label{2}
    \ndl{}{\(\neg\psi \to (\phi \to \neg\psi)\)}{\(\rm P_1\)}\label{3}
    \ndl{}{\((\neg\psi \to (\phi \to \neg\psi)) \to (\neg\psi \to \neg(\phi \to \neg\psi)) \to \psi\)}{\(\rm P_3\)}\label{4}
    \ndl{}{\(\neg\psi \to \neg(\phi \to \neg\psi)\)}{\ref{2}，演绎\oldref{ded:axiom1}}\label{5}
    \ndl{}{\((\neg\psi \to \neg(\phi \to \neg\psi)) \to \psi\)}{\ref{3}，\ref{4}，MP}\label{6}
    \ndl{}{\(\psi\)}{\ref{5}，\ref{6}，MP}
  \end{ND}
\item \label{ded:wedgeOutLeft} \(\phi \land \psi \proves \phi\)
  \begin{ND}[][][][\rwidth{ded:wedgeComm1}]
    \ndl{}{\(\phi \land \psi\)}{假设}\label{1}
    \ndl{}{\(\neg(\phi \to \neg\psi)\)}{\ref{1}，定义2.2.4}\label{2}
    \ndl{}{\(\phi \to \neg\phi \to \neg\psi\)}{证明\oldref{thm:exFalso}}\label{3}
    \ndl{}{\(\neg\phi \to (\phi \to \neg\psi)\)}{\ref{3}，演绎\oldref{ded:comm}}\label{4}
    \ndl{}{\((\neg\phi \to (\phi \to \neg\psi)) \to (\neg\phi \to \neg(\phi \to \neg\psi)) \to \phi\)}{\(\rm P_3\)}\label{5}
    \ndl{}{\(\neg\phi \to \neg(\phi \to \neg\psi)\)}{\ref{2}，演绎\oldref{ded:axiom1}}\label{6}
    \ndl{}{\((\neg\phi \to \neg(\phi \to \neg\psi)) \to \phi\)}{\ref{4}，\ref{5}，MP}\label{7}
    \ndl{}{\(\phi\)}{\ref{6}，\ref{7}，MP}
  \end{ND}
\item \label{ded:wedgeComm} \(\phi \land \psi \proves \psi \land \phi\)
  \begin{ND}[][ded:wedgeComm1]
    \ndl{}{\(\phi \land \psi\)}{假设}\label{1}
    \ndl{}{\(\psi\)}{\ref{1}，演绎\oldref{ded:wedgeOutRight}}\label{2}
    \ndl{}{\(\phi\)}{\ref{1}，演绎\oldref{ded:wedgeOutLeft}}\label{3}
    \ndl{}{\(\psi \land \phi\)}{\ref{2}，\ref{3}，演绎\oldref{ded:wedgeIn}}
  \end{ND}
  或者
  \begin{ND}[][][][\rwidth{ded:wedgeComm1}]
    \ndl{}{\(\phi \land \psi\)}{假设}\label{1}
    \ndl{}{\(\neg(\phi \to \neg\psi)\)}{\ref{1}，定义2.2.4}\label{2}
    \ndl{}{\((\psi \to \neg\phi) \to (\neg\neg\psi \to \neg\phi)\)}{证明\oldref{thm:dnInAnte}}\label{3}
    \ndl{}{\((\neg\neg\psi \to \neg\phi) \to (\phi \to \neg\psi)\)}{证明\oldref{thm:axiom3alt}}\label{4}
    \ndl{}{\((\psi \to \neg\phi) \to (\phi \to \neg\psi)\)}{\ref{3}，\ref{4}，演绎\oldref{ded:trans}}\label{5}
    \ndl{}{\(((\psi \to \neg\phi) \to (\phi \to \neg\psi))
      \to ((\psi \to \neg\phi) \to \neg(\phi \to \neg\psi))
      \to \neg(\psi \to \neg\phi)\)}{证明\oldref{thm:axiom3in}}\label{6}
    \ndl{}{\((\psi \to \neg\phi) \to \neg(\phi \to \neg\psi)\)}{\ref{2}，演绎\oldref{ded:axiom1}}\label{7}
    \ndl{}{\(((\psi \to \neg\phi) \to \neg(\phi \to \neg\psi))
      \to \neg(\psi \to \neg\phi)\)}{\ref{5}，\ref{6}，MP}\label{8}
    \ndl{}{\(\neg(\psi \to \neg\phi)\)}{\ref{7}，\ref{8}，MP}\label{9}
    \ndl{}{\(\psi \land \phi\)}{\ref{9}，定义2.2.4}
  \end{ND}
\item \label{ded:veeInRight} \(\phi \proves \phi \lor \psi\)
  \begin{ND}[][][][\rwidth{ded:wedgeComm1}]
    \ndl{}{\(\phi\)}{假设}\label{1}
    \ndl{}{\(\phi \to \neg\phi \to \psi\)}{证明\oldref{thm:exFalso}}\label{2}
    \ndl{}{\(\neg\phi \to \psi\)}{\ref{1}，\ref{2}，MP}\label{3}
    \ndl{}{\(\phi \lor \psi\)}{\ref{3}，定义2.2.4}
  \end{ND}
\item \label{ded:veeComm} \(\phi \lor \psi \proves \psi \lor \phi\)
  \begin{ND}[][][][\rwidth{ded:wedgeComm1}]
    \ndl{}{\(\phi \lor \psi\)}{假设}\label{1}
    \ndl{}{\(\neg\phi \to \psi\)}{\ref{1}，定义2.2.4}\label{2}
    \ndl{}{\(\neg\phi \to \neg\neg\psi\)}{\ref{2}，演绎\oldref{ded:dnInConseq}}\label{3}
    \ndl{}{\((\neg\phi \to \neg\neg\psi) \to (\neg\psi \to \phi)\)}{证明\oldref{thm:axiom3alt}}\label{4}
    \ndl{}{\(\neg\psi \to \phi\)}{\ref{3}，\ref{4}，MP}\label{5}
    \ndl{}{\(\psi \lor \phi\)}{\ref{5}，定义2.2.4}
  \end{ND}
\item \label{ded:veeInLeft} \(\phi \proves \psi \lor \phi\)
  \begin{ND}[][][][\rwidth{ded:wedgeComm1}]
    \ndl{}{\(\phi\)}{假设}\label{1}
    \ndl{}{\(\phi \lor \psi\)}{\ref{1}，演绎\oldref{ded:veeInRight}}\label{2}
    \ndl{}{\(\psi \lor \phi\)}{\ref{2}，演绎\oldref{ded:veeComm}}
  \end{ND}
\item \label{ded:veeOutRight} \(\phi \lor \psi, \neg\phi \proves \psi\)
  \begin{ND}[][][][\rwidth{ded:wedgeComm1}]
    \ndl{}{\(\phi \lor \psi\)}{假设}\label{1}
    \ndl{}{\(\neg\phi\)}{假设}\label{2}
    \ndl{}{\(\neg\phi \to \psi\)}{\ref{1}，定义2.2.4}\label{3}
    \ndl{}{\(\psi\)}{\ref{2}，\ref{3}，MP}
  \end{ND}
\item \label{ded:veeOutLeft} \(\phi \lor \psi, \neg\psi \proves \phi\)
  \begin{ND}[][][][\rwidth{ded:wedgeComm1}]
    \ndl{}{\(\phi \lor \psi\)}{假设}\label{1}
    \ndl{}{\(\neg\psi\)}{假设}\label{2}
    \ndl{}{\(\psi \lor \phi\)}{\ref{1}，演绎\oldref{ded:veeComm}}\label{3}
    \ndl{}{\(\neg\psi \to \phi\)}{\ref{3}，定义2.2.4}\label{4}
    \ndl{}{\(\psi\)}{\ref{2}，\ref{4}，MP}
  \end{ND}
\end{enumerate}

\end{document}

% Local Variables:
% TeX-engine: luatex
% End:
